src/ReactorModel/Objects/Reactor/Theorems/LawfulUpdate.lean
@@ -9,28 +9,39 @@ theorem UniqueIDs.updated [ReactorType.WellFounded α] {rtr₁ rtr₂ : α}
       |>.trans (Equivalent.from_lawfulUpdate u m₂).symm 
       |>.to_eq
 
-theorem LawfulMemUpdate.member₁ [ReactorType α] {rtr₁ rtr₂ : α}
+def LawfulMemUpdate.member [ReactorType α] {rtr₁ rtr₂ : α}
     (u : LawfulMemUpdate cpt i f rtr₁ rtr₂) : Member cpt i rtr₁ :=
   sorry
 
-theorem LawfulMemUpdate.member₂ [ReactorType α] {rtr₁ rtr₂ : α}
-    (u : LawfulMemUpdate cpt i f rtr₁ rtr₂) : Member cpt i rtr₂ :=
-  sorry -- by u.member₁ and u.equiv
+def LawfulMemUpdate.unique [Indexable α] {rtr rtr₁ rtr₂ : α}
+    (u₁ : LawfulMemUpdate cpt i f rtr rtr₁) (u₂ : LawfulMemUpdate cpt i f rtr rtr₂) : rtr₁ = rtr₂ := 
+  sorry 
 
-theorem LawfulUpdate.ne_comm [ReactorType α] {rtr rtr₁ rtr₁' rtr₂ rtr₂' : α} 
+theorem LawfulMemUpdate.ne_comm [Indexable α] {rtr rtr₁ rtr₁' rtr₂ rtr₂' : α} 
+    (u₁ : LawfulMemUpdate cpt₁ i₁ f₁ rtr rtr₁) (u₂ : LawfulMemUpdate cpt₂ i₂ f₂ rtr₁ rtr₂) 
+    (u₁' : LawfulMemUpdate cpt₂ i₂ f₂ rtr rtr₁') (u₂' : LawfulMemUpdate cpt₁ i₁ f₁ rtr₁' rtr₂') 
+    (h : cpt₁ ≠ cpt₂ ∨ i₁ ≠ i₂) : rtr₂ = rtr₂' := by
+  sorry
+
+theorem LawfulUpdate.ne_comm [Indexable α] {rtr rtr₁ rtr₁' rtr₂ rtr₂' : α} 
     (u₁ : LawfulUpdate cpt₁ i₁ f₁ rtr rtr₁) (u₂ : LawfulUpdate cpt₂ i₂ f₂ rtr₁ rtr₂) 
     (u₁' : LawfulUpdate cpt₂ i₂ f₂ rtr rtr₁') (u₂' : LawfulUpdate cpt₁ i₁ f₁ rtr₁' rtr₂') 
     (h : cpt₁ ≠ cpt₂ ∨ i₁ ≠ i₂) : rtr₂ = rtr₂' := by
-  cases u₁ <;> cases u₂' <;> cases u₂ <;> cases u₁'
-  case update.update.update.notMem =>
-    exact IsEmpty.elim ‹_› $ sorry
-    -- have := LawfulMemUpdate.member ‹_›  
-  all_goals sorry -- The only cases that should remain have matching kind on u₁&u₂' and u₂&u₁':
-            -- nnnn, nnuu, uunn, uuuu
-  -- Can you prove this without extensionality?
+  cases u₁ <;> cases u₂' <;> cases u₁' <;> cases u₂ <;> repeat subst ‹_ = _›
+  case update.update.update.update u₁ u₂' u₁' u₂ => exact LawfulMemUpdate.ne_comm u₁ u₂ u₁' u₂' h
+  case notMem.notMem.notMem.notMem => rfl
+  case notMem.notMem.update.update => exact LawfulMemUpdate.unique ‹_› ‹_› 
+  case update.update.notMem.notMem => exact LawfulMemUpdate.unique ‹_› ‹_› 
+  all_goals first 
+    | exact IsEmpty.elim ‹_› $ LawfulMemUpdate.member ‹_›
+    | refine IsEmpty.elim ‹_› ?_
+      try exact LawfulMemUpdate.member ‹_›
+      try exact .fromEquiv (LawfulMemUpdate.equiv ‹_›) $ LawfulMemUpdate.member ‹_›
+  case update.update.notMem.update u' _ u  _ => exact .fromEquiv (Equivalent.symm u'.equiv) u.member
+  case notMem.update.update.update _  u u' _ => exact .fromEquiv (Equivalent.symm u'.equiv) u.member
 
 open Updatable in
-theorem LawfulUpdatable.update_ne_comm [LawfulUpdatable α] {rtr : α} (h : cpt₁ ≠ cpt₂ ∨ i₁ ≠ i₂):
+theorem LawfulUpdatable.update_ne_comm [Indexable α] {rtr : α} (h : cpt₁ ≠ cpt₂ ∨ i₁ ≠ i₂):
     update (update rtr cpt₁ i₁ f₁) cpt₂ i₂ f₂ = update (update rtr cpt₂ i₂ f₂) cpt₁ i₁ f₁ :=
   LawfulUpdate.ne_comm (lawful ..) (lawful ..) (lawful ..) (lawful ..) h
   
